\documentclass{beamer}
% Theme choice:
\usetheme{CambridgeUS}
% Title page details: 
\title{Assignment-8} 
\author{Nwjwr Khungur Brahma (AI20BTECH11016)}
\date{\today}
\newcounter{currentenumi}
\begin{document}

\begin{frame}
\titlepage
\end{frame}

\begin{frame}{Outline}
\tableofcontents
\end{frame}

\section{Question}
\begin{frame}{Question}
$x$ and $y$ are independent identically distributed normal random variables with zero mean and common variance $\sigma^{2}$, that is, $x  \sim N(0,\sigma^{2}),$ $y \sim N(0,\sigma^{2})$ and $f_{xy}(x,y)= f_x(x).f_y(y).$\\
Find the pdf of
\begin{enumerate}
\item $x$ = $\sqrt{x^{2}+y^{2}}$
\item $w$ = $x^{2}+y^{2}$
\item $u$ = $x - y$
\end{enumerate}
\end{frame}

\section{Solution}
\begin{frame}{Solution}
\begin{enumerate}
\item For $z$ = $\sqrt{x^{2}+y^{2}}$\\ 
The case corresponds to a circle with radius $z$. Thus
\begin{align}
F_z(z)= \int_{y=\text{-}z}^{z} \int_{x=\text{-}\sqrt{z^{2}-y^{2}}}^{\sqrt{z^{2}-y^{2}}} f_{xy}(x,y)\,dx \,dy
\end{align}
and by differentiation,
\begin{align}
f_z(z)= \int_{-z}^{z} \frac{z}{\sqrt{z^{2}-y^{2}}} \left(f_{xy}(\sqrt{z^{2}-y^{2}},y)+f_{xy}(\text{-}\sqrt{z^{2}-y^{2}},y)\right) \,dy
\end{align}
As $x$ and $y$ are zero mean independent Gaussian random variables with common variance $\sigma^{2}$
\begin{align}
f_z(z)= 2 \int_{0}^{z} \frac{z}{\sqrt{z^{2}-y^{2}}}\frac{2}{2 \pi \sigma^{2}} \exp^{\frac{\text{-}(z^{2}-y^2+y^2)}{2 \sigma^2}} \,dy
\end{align}
\setcounter{currentenumi}{\theenumi}
\end{enumerate}
\end{frame}

\begin{frame}
\begin{align}
&=\frac{2z}{\pi \sigma^2} \exp^{\text{-}\frac{z^2}{2\sigma^2}} \int_0^z \frac{1}{\sqrt{z^2-y^2}} \,dy\\
&=\frac{2z}{\pi \sigma^2} \exp^{\frac{\text{-}z^2}{2 \sigma^2}} \int_0^{\frac{\pi}{2}} \frac{z \cos \theta}{z \cos \theta} \,d\theta\\
&=\frac{2z}{\pi \sigma^2} \exp^{\frac{\text{-}z^2}{2 \sigma^2}}U(z)
\end{align}
\end{frame}

\begin{frame}
\begin{enumerate}
\setcounter{enumi}{\thecurrentenumi}
\item We know that for $z$ = $\sqrt{x^{2}+y^{2}}$
\begin{align}
f_z(z)= \int_{-z}^{z} \frac{z}{\sqrt{z^{2}-y^{2}}} \left(f_{xy}(\sqrt{z^{2}-y^{2}},y)+f_{xy}(\text{-}\sqrt{z^{2}-y^{2}},y)\right) \,dy
\end{align}
As $w = x^2 + y^2$, x and y are independent random variables with zero mean and common variance $\sigma^{2}$.
\begin{align}
f_w(w)&= \int_{\text{-}\sqrt{w}}^{\sqrt{w}} \frac{1}{2 \sqrt{w-y^2}} \left(2.\frac{1}{2 \pi \sigma^{2}} \exp^{(\frac{w-y^{2}+y^{2}}{2 \sigma^{2}})}\right) \,dy\\
&=\frac{\exp^{\frac{\text{-}w}{2\sigma^{2}}}}{\pi \sigma^{2}} \int_{0}^{\sqrt{w}}\frac{1}{\sqrt{w-y^{2}}} \,dy\\
&=\frac{\exp^{\frac{\text{-}w}{2\sigma^{2}}}}{\pi \sigma^{2}} \int_{0}^{\frac{\pi}{2}} \frac{\sqrt{w}\cos \theta}{\sqrt{w}\cos \theta} \,d\theta\\
&=\frac{1}{2 \sigma^{2}} \exp^{\frac{\text{-}w}{2 \sigma^{2}}} U(w)
\end{align}
\setcounter{currentenumi}{\theenumi}
\end{enumerate}
\end{frame}

\begin{frame}
\begin{enumerate}
\setcounter{enumi}{\thecurrentenumi}
\item For $u = x-y$\\
Since linear combinations of jointly Gaussian random variables are Gaussian random Variables. Here $var(u)= var(x) + var(y) = 2\sigma^2$\\
So $u = x-y \sim N(0,2\sigma^2)$\\
\begin{align}
f_u(u)&= \int_{\text{-} \infty}^{\infty} f_x(z+y)f_y(y)\,dy
\end{align}
\end{enumerate}
\end{frame}
\end{document}